$\frac{d \vec{p}}{dt}= \vec{F}$
$\vec{p}= \frac{m\vec{v}}{\sqrt{ 1-\left( \frac{v}{c} \right)^2 }}$
$\frac{d}{dt}\left( \frac{m\vec{v}}{\sqrt{ 1-\left( \frac{v}{c} \right)^2 }} \right)=\vec{F}$
$\vec{p}=m\vec{v}$
$m=\frac{m_{0}}{\sqrt{ 1-\left( \frac{v}{c} \right)^2 }}=m(v)=f(v)$
$\frac{d(m\vec{v})}{dt}=\frac{dm}{dt}^\vec{v}+\frac{md\vec{v}}{dt}=\vec{F}$
![[Pasted image 20240418185503.png]](2=$\frac{d\vec{v}}{dt}m$),(1=$\frac{dm}{dt}*\vec{v}$)
$\vec{F} \uparrow\uparrow \vec{a}$ - поперечная сила
1) $\vec{F} \perp \vec{v}$
2) $\vec{F}\uparrow\uparrow \vec{v}$ - продольная сила
3) $\vec{F}\downarrow\uparrow \vec{v}$

$\frac{d}{dt}\left( \frac{m\vec{v}}{\sqrt{ 1-\left( \frac{v}{c} \right)^2 }} \right)=\frac{m_{0}* \frac{dv}{dt}}{\sqrt{ 1-\left( \frac{v}{c} \right)^2 }}+ \frac{m_{0}v\left(\frac{-2v}{c^2} \right) *\left( \frac{1}{2} \right)}{\left( 1-\frac{v}{c} \right)^{3/2}}* \frac{dv}{dt}= m_{0} * \frac{dv}{dt}\left( \frac{1}{\sqrt{ 1-\left( \frac{v}{c} \right)^2 }} +\frac{\frac{v^2}{c^2}}{\left( 1-\left( \frac{v}{c} \right)^2 \right)^{3/2}} \right)=m_{0}* \frac{dv}{dt}\left( \frac{1-\left( \frac{v}{c} \right)^2 +\left( \frac{v}{c} \right)^2}{\left( 1-\left( \frac{v}{c} \right)^2 \right)^{3/2}} \right)=m_{0} \frac{dv}{dt* \frac{1}{\left( 1-\left( \frac{v}{c} \right)^2 \right)^{3/2}}}\implies a= \frac{dv}{dt}=\frac{F}{m_{0}}*\left( 1-\left( \frac{v}{c} \right)^2 \right)^{3/2}$
$dA=Fds= \frac{mdv}{dt}vdt=mvdv=d\left( \frac{mv^2}{2} \right)$
$dA=Fds=\frac{dp}{dt}vdt=d\left( \frac{m_{0}v}{\sqrt{ 1-\left( \frac{v}{c} \right)^2 }} \right)v=v* \frac{m_{0}dv}{\left( 1-\left( \frac{v}{c} \right)^2 \right)^{3/2}}=\frac{1}{2}* \frac{dm_{0}v^2}{\left( 1-\left( \frac{v}{c} \right)^2 \right)^{3/2}}= d()$
$\frac{m_{0}C^2}{2} \frac{dx^2}{(1-x^2)^{3/2}}=\frac{m_{0}c^2}{2} \frac{dy}{(1-y)^{3/2}}=\frac{m_{0}c^2}{2} \frac{d(1-y)}{(1-y)^{3/2}}=O \frac{dz}{z^{3/2}}=dz*z^{-3/2}=\frac{m_{0}c^2}{2}d(\left( \frac{(1-y)^{-1/2}}{-\frac{1}{2}} \right)=m_{0}c^2d\left( 1-\left( \frac{v}{c} \right) \right)^{-1/2}=d\left( \frac{m_{0}c^2}{1-\left( \frac{v}{c} \right)^2} \right)=\underset{ dA=dF_{k} }{ dE_{k} }$
$E_{k}(v)=\frac{m_{0}c^2}{\sqrt{ 1-\left( \frac{v}{c} \right)^2 }}+ const$

$E_{k}(0)\neq 0$(так не должно быть)
$E_{k}(0)=0= \frac{m_{0}c^2}{\sqrt{ 1-o^2 }}+vonst \implies const=-m_{0}c^2$
$E_{k}=m_{0}c^2\left( \frac{1}{\sqrt{ 1-\left( \frac{v}{c} \right)^2 }} -1 \right)$
$\frac{1}{\sqrt{ 1-\beta^2 }}=(1-\beta^2)^{-1/2}\approx \underset{ b\to_{0}(v\ll c) }{ 1+\frac{1}{2} \beta^2+\frac{3}{8}\beta^4 }$
$\underset{ v\ll c }{ E_{k}=m_{0}c^2 }\left( 1+\frac{1}{2}\left( \frac{v}{c} \right)^2+\dots-1 \right)=\frac{1}{2}m_{0}c^2* \frac{v^2}{c^2}=\frac{m_{0}v^2}{2}$
$\underset{ \text{полная энергия} }{ E }= E_{k}+E_{0}$
$E_{0}=m_{0}c^2$
$E = \frac{m_{0}c^2}{\sqrt{ 1-\left( \frac{v}{c} \right)^2 }}-m_{0}c^2+m_{0}c^2$
$E_{k}=E-E_{0}=\frac{m_{0}c^2}{\sqrt{ 1-\left( \frac{v}{c} \right)^2 }}-m_{0}c^2$
$E^2-p^2c^2=\underset{ инвариантность }{ inv }$
$\frac{m_{0}^2c^4}{\left( 1-\left( \frac{v}{c} \right)^2 \right)}-\frac{m_{0}^2v^2c^2}{\left( 1-\left( \frac{v}{c} \right)^2 \right)}=\frac{m_{0}c^4}{1-\left( \frac{v}{c} \right)^2}*\left( 1+\frac{v^2}{c^2} \right)=m_{0}^2c^4$
$E^2-p^2c^2=m_{0}^2c^4$

$m_{0}=0$
$E^2=p^2c^2$
$p_{\phi}=\frac{E}{c}$ 
![[IMG_20240418_201914.jpg]](сверху написано "линии тока")(снизу написано "течение стационарное")

![[IMG_20240418_201921.jpg]]

$\int_{1}^{\infty} \cos\left( \frac{\pi}{3} \right) \, d\pi$

