$x(t) = A\cos(w_{0}+\phi_{0})$; $v(t)=Aw_{0}\sin(w_{0}t+\phi_{0})$
$E_{k}(t)=\frac{mv^2(t)}{2}=\frac{mA^2w^2_{0}}{2}\sin^2(w_{0}t+\phi_{0})$
$E_{n}(t)=\frac{kx(t)^2}{2}=\frac{kA^2\cos^2(w_{0}+\phi_{0})}{2}$
$E=E_{k}(t)E_{n}(t)=\frac{mA^2w_{0}^2}{2}\sin^2(w_{0}t+\phi_{0})+\frac{kA^2}{2}\cos^2(w_{0}t+\phi_{0})= \frac{kA^2}{2}\sin^2(w_{0}+\phi_{0})+\frac{kA^2}{2}\cos^2(w_{0}t+\phi_{0})=\frac{kA^2}{2}=\frac{mw_{0}^2A^2}{2}$
$E=E_{k \ max}=E_{n \ max}$
$E = \frac{kA^2}{2}=\frac{mw_{0}A^2}{2}$
![[Pasted image 20240314185646.png]]
![[Pasted image 20240314185944.png]]

## Квазиупругие силы
$F = -kx$;     ($mx'' = -kx$)
![[Pasted image 20240314190821.png]](тут $l$ похожа на $e$)
$\sin \alpha = \frac{x}{l}$
$ma = -mg \frac{x}{l}$; $\frac{mg}{l} = k$
$mx'' = -\frac{mg}{e} * x$
$\omega_{0} = \sqrt{ \frac{k}{m} }=\sqrt{ \frac{g}{l} }$
$T= \frac{2\pi}{\omega_{0}}=2\pi \sqrt{ \frac{l}{g} }$
## Сложение колебаний
$x(t)= A \cos(\omega_{0}+\phi_{0})$
![[Pasted image 20240314191925.png]]
$A_{x}(t)=A\cos(\omega_{0}t+\phi_{0})=x(t)$
![[Pasted image 20240314192317.png]]
$A^2=A_{1}^2+A_{2}^2-2A_{1}A_{2}\cos \beta = A_{1}^2+A_{2}^2\cos(\pi - (\phi_{02}-\phi_{01}))$; $\beta = \pi - (\phi_{02} - \phi_{01})$
$A^2 = A_{1}^2+A_{2}^2 + 2A_{1}A_{2}\cos(\phi_{02}-\phi_{01})$
$\nabla \phi = \mid \phi_{02} - \phi_{01} \mid$ - разность

$A_{1}=A_{2}=A_{0}$
$A^2=2A_{0}^2(1+\cos \nabla \phi)$
1) $\nabla \phi = 0$
	$A^2=2A^2_{0}(1+1)=4A_{0}^2$
	$A=2A_{0}$
2) $\nabla \phi = \pi$
	$A^2=2A_{0}^2(1-1)=0$;  $A=0$
	![[Pasted image 20240314193001.png]]

![[Pasted image 20240314193058.png]]

## сложение взаимноперпендикулярных колебаний
$x(t) = A_{1}\cos (\omega_{0}t+\phi_{0})$
$y(t) = A_{2}\cos(\omega_{0}t)$
1) $\phi_{0}=0$
	 $\frac{x}{y}=\frac{A_{1}}{A_{2}} \to \ y-\frac{A_{2}}{A_{2}}x_{1}$
	 ![[Pasted image 20240314194041.png]]
2) $\phi_{0}=\frac{\pi}{2}$
	$x(t)=A_{1}\cos\left( \omega_{0}t+\frac{\pi}{2} \right)=-A_{1}\sin(\omega_{0}t)$
	$y(t)=A_{2}\cos(\omega_{0}t)$
	$\frac{x^2}{A_{1}^2} + \frac{y^2}{A_{1}^2} = 1$
	![[Pasted image 20240314194452.png]]
3) $\phi_{0}=\pi$
	$x(t)=-A_{1}\cos(\omega_{0}t)$
	y(t) = $A_{2}\cos(\omega_{0}t)$
	$y=-\frac{A_{2}}{A_{2}}x$
	![[Pasted image 20240314194518.png]]
$\phi_{0}=\frac{\pi}{2}$
$\omega_{0x}=\omega_{0}$;  $\omega_{0y}=2\omega_{0}$
$x(t) = -A_{1}\sin \omega_{0}t$
$y(t)=A_{2}\cos(2\omega_{0}t)=A_{2}(\cos^2(\omega t)-\sin^2\omega_{0}t)=A_{2}\left( 1-\frac{x^2}{A_{1}^2} -\frac{x^2}{A_{1}^2}\right)=A_{2}\left( 1-\frac{2x^2}{A_{1}^2} \right)$
![[Pasted image 20240314194936.png]]
$x(t)=A\sin(\omega t)$
$y(t)=A_{2}\sin(2\omega_{0} t)=2A_{2}\sin(\omega_{0}t)\cos(\omega_{0}t)$
$y(x)=2A_{2} \frac{x}{A_{1}}*\pm\sqrt{ 1-\frac{x^2}{A_{1}^2} }$
cos=($\pm \sqrt{  }$)
![[Pasted image 20240314195328.png]]
## Затухающие колебания
$ma_{x} = -kx -rv$
$mx'' = -kx -rx'$
$mx'' + rx' + kx=0$;   $\omega_{0}^2= \frac{k}{m}$
$x'' = \frac{r}{m}x'+\frac{kx}{m}=0$;   $2\beta = \frac{r}{m}$ 
$x'' = 2\beta x' + \omega_{0}^2x=0$
$x(t)= A_{0}e^{-\beta t}*\cos(\omega t+\phi_{9})$
$\omega=\sqrt{ \omega_{0}^2-\beta^2 }$;   $\beta$ - коэффициент затухания
$T = \frac{2\pi}{\sqrt{ w_{0}^2  - \beta^2}}$
{${\beta}$} = $c^{-1}$
![[Pasted image 20240314201219.png]]
$\beta=\frac{r}{2m}$
$\lambda = \ln \frac{A(t)}{A(t+ \mathcal{T})}$ 
$\lambda = \ln \frac{A_{0}*e^{-\beta t}}{A_{0}*e^{-\beta(t+\mathcal{T})}}=\ln \ e^{-\beta t + \beta t \mathcal{T}}= \ln \ E^{\beta \mathcal{T}}$
$\lambda = \beta * \mathcal{T}$
